fix: add step cost

Reap/Test/Tactic/MCTS.lean
@@ -14,8 +14,15 @@ def andOrTacGen : TacGen := fun _ => do
 def andOrStateEval : StateEval := fun _ => do
   return 0.0
 
-example : (a b c : Nat) → a = b → b = c → a = c := by
-  reapMCTS
+def transTacGen : TacGen := fun _ => do
+  return #[
+    ("trans b", #[], 1.0),
+    ("exact h1", #[], 1.0),
+    ("exact h2", #[], 1.0)
+  ]
+
+example (a b c : Nat) (h1 : a = b) (h2 : b = c) : a = c := by
+  run_tac reapMCTS transTacGen andOrStateEval (maxNodes := 32) (maxSteps := 32)
 
 example (P Q : Prop) (hP : P) (hQ : Q) : P ∧ Q := by
   run_tac reapMCTS andOrTacGen andOrStateEval (maxNodes := 32) (maxSteps := 32)
